src/prototype/Example4.v
@@ -1,0 +1,29 @@
+Require Import Vector.
+Import Vector.VectorNotations.
+
+Inductive instr :=
+  | A : instr
+  | B : instr
+  | C : instr.
+
+
+Definition vector_zip {A B : Type} {n : nat} (v1 : Vector.t A n)
+                      (v2 : Vector.t B n) : Vector.t (A * B) n :=
+  Vector.map2 (fun x y => (x, y)) v1 v2.
+
+Check (5,5).
+
+Fixpoint f' {n} (L : Vector.t (instr*instr) n) : Vector.t instr n :=
+  match L with
+  | [] => []
+  | (A,h)::L' => h :: f' L'
+  | (a,_)::L' => a :: f' L'
+  end.
+
+Definition f {n} (l : Vector.t instr n) (m : Vector.t instr n) :
+                   Vector.t instr n := f' (vector_zip l m).
+
+
+
+Theorem th : forall p ind, p[@ind] <> A ->
+                           f p 
